Upgrade DSL to work in type position

formal/SkLean/Ast3.lean
@@ -8,9 +8,11 @@ inductive Expr where
   | s    : Expr
   | m    : Expr
   | arr  : Expr
-  | ty   : ℕ → Expr
   | call : Expr → Expr → Expr
 deriving BEq, Repr, Lean.ToExpr
+
+inductive ExprBox (e : Ast.Expr) where
+  | mk : ExprBox e
 
 declare_syntax_cat skmexpr
 syntax "K"                     : skmexpr
@@ -20,21 +22,21 @@ syntax "#~>"                   : skmexpr
 syntax skmexpr "~>" skmexpr    : skmexpr
 syntax "(" skmexpr skmexpr ")" : skmexpr
 syntax ident                   : skmexpr
-syntax "Ty" term               : skmexpr
 syntax "#" term                : skmexpr
 syntax "(" skmexpr ")"         : skmexpr
 
 syntax " ⟪ " skmexpr " ⟫ "     : term
 syntax "SKM[ " skmexpr " ] "   : term
+syntax "SKM'[ " skmexpr " ] "  : term
 
 macro_rules
-  | `(SKM[ $e:skmexpr ]) => `(⟪ $e ⟫)
+  | `(SKM[ $e:skmexpr ])  => `(⟪ $e ⟫)
+  | `(SKM'[ $e:skmexpr ]) => `(ExprBox ⟪ $e ⟫)
 
 macro_rules
   | `(⟪ K ⟫)                           => `(Expr.k)
   | `(⟪ S ⟫)                           => `(Expr.s)
   | `(⟪ M ⟫)                           => `(Expr.m)
-  | `(⟪ Ty $n:term ⟫)                  => `(Expr.ty $n)
   | `(⟪ #~> ⟫)                         => `(Expr.arr)
   | `(⟪ $e₁:skmexpr ~> $e₂:skmexpr ⟫)  => `(Expr.call (Expr.call Expr.arr ⟪ $e₁ ⟫) ⟪ $e₂ ⟫)
   | `(⟪ $e:ident ⟫)                    => `($e)
@@ -53,7 +55,6 @@ def toStringImpl (e : Expr) : String :=
   | SKM[((t_in ~> t_out) ~> t₃)] => s!"({t_in.toStringImpl} → {t_out.toStringImpl}) → {t₃.toStringImpl}"
   | SKM[(t_in ~> t_out)] => s!"{t_in.toStringImpl} → {t_out.toStringImpl}"
   | SKM[(lhs rhs)] => s!"({lhs.toStringImpl} {rhs.toStringImpl})"
-  | SKM[Ty n] => s!"Type {n}"
 
 instance : ToString Expr where
   toString := toStringImpl
@@ -63,7 +64,6 @@ def fromExpr (e : Lean.Expr) : Option Expr :=
   | .const `Expr.k [] => pure SKM[K]
   | .const `Expr.s [] => pure SKM[S]
   | .const `Expr.m [] => pure SKM[M]
-  | .app (.const `Expr.ty []) (.lit (.natVal n)) => pure SKM[Ty n]
   | .const `Expr.arr [] => pure SKM[#~>]
   | .app (.app (.const `Expr.call []) lhs) rhs => do
     let lhs' ← fromExpr lhs
