formal/SkLean/Translator.lean
@@ -1,6 +1,5 @@
 import Lean
 import SkLean.Ast3
-import SkLean.UnsafeEval
 import SkLean.Eval
 import SkLean.Checker
 open Lean
@@ -41,7 +40,6 @@ syntax "#~>"                      : skmexpr'
 syntax skmexpr' "~>" skmexpr'     : skmexpr'
 syntax "(" skmexpr' skmexpr' ")"  : skmexpr'
 syntax ident                      : skmexpr'
-syntax "Ty" term                  : skmexpr'
 syntax "#" term                   : skmexpr'
 syntax "(" skmexpr' ")"           : skmexpr'
 syntax "λ" skmexpr' "=>" skmexpr' : skmexpr'
@@ -49,17 +47,16 @@ syntax "∀" skmexpr' "," skmexpr'  : skmexpr'
 syntax "!" skmexpr'               : skmexpr'
 
 syntax " {{ " skmexpr' " }} "     : term
-syntax "SKM'[ " skmexpr' " ] "    : term
+syntax "SKM`[ " skmexpr' " ] "    : term
 
 macro_rules
-  | `(SKM'[ $e:skmexpr' ]) => `({{ $e }})
+  | `(SKM`[ $e:skmexpr' ]) => `({{ $e }})
 
 macro_rules
   | `({{ !$e:skmexpr' }})                    => `(IntermediateExpr.intr {{ $e }})
   | `({{ K }})                               => `(IntermediateExpr.k)
   | `({{ S }})                               => `(IntermediateExpr.s)
   | `({{ M }})                               => `(IntermediateExpr.m)
-  | `({{ Ty $n:term }})                      => `(IntermediateExpr.ty $n)
   | `({{ λ $t:skmexpr' => $body:skmexpr' }}) => `(IntermediateExpr.lam {{$t}}  {{$body}})
   | `({{ ∀ $t:skmexpr', $body:skmexpr' }})   => `(IntermediateExpr.forE {{$t}} {{$body}})
   | `({{ #~> }})                             => `(IntermediateExpr.arr)
@@ -73,67 +70,70 @@ namespace IntermediateExpr
 
 def all_human_sk (e : IntermediateExpr) : Bool :=
   match e with
-  | SKM'[S]         => true
-  | SKM'[K]         => true
-  | SKM'[M]         => true
-  | SKM'[Ty n]      => true
-  | SKM'[(lhs rhs)] => all_human_sk lhs ∧ all_human_sk rhs
-  | SKM'[#~>]       => true
+  | SKM`[S]         => true
+  | SKM`[K]         => true
+  | SKM`[M]         => true
+  | SKM`[(lhs rhs)] => all_human_sk lhs ∧ all_human_sk rhs
+  | SKM`[#~>]       => true
   | _               => false
 
 def all_sk (e : IntermediateExpr) : Option Ast.Expr :=
   match e with
   | .skm e          => pure e
-  | SKM'[S]         => pure SKM[S]
-  | SKM'[K]         => pure SKM[K]
-  | SKM'[M]         => pure SKM[M]
-  | SKM'[Ty n]      => pure SKM[Ty n]
-  | SKM'[(lhs rhs)] => do
+  | SKM`[S]         => pure SKM[S]
+  | SKM`[K]         => pure SKM[K]
+  | SKM`[M]         => pure SKM[M]
+  | SKM`[(lhs rhs)] => do
     let lhs' ← lhs.all_sk
     let rhs' ← rhs.all_sk
 
     pure SKM[(lhs' rhs')]
-  | SKM'[#~>] => SKM[#~>]
+  | SKM`[#~>] => SKM[#~>]
   | .intr e => e.all_sk
   | _ => .none
 
 def from_expr : Lean.Expr → Except Lean.Expr IntermediateExpr
+  | (.app (.const `Ast.ExprBox []) e) => from_expr e
   | .bvar n           => pure $ .var n
-  | .const `Expr.k [] => pure SKM'[S]
-  | .const `Expr.s [] => pure SKM'[K]
-  | .const `Expr.m [] => pure SKM'[M]
-  | (.app (.const `Expr.ty []) (.lit (.natVal n))) => pure $ .ty n
-  | .const `Expr.arr [] => pure SKM'[#~>]
-  | .sort t             => pure $ SKM'[Ty (t.depth.pred)]
+  | .const `Ast.Expr.k [] => pure SKM`[K]
+  | .const `Ast.Expr.s [] => pure SKM`[S]
+  | .const `Ast.Expr.m [] => pure SKM`[M]
+  | (.app (.const `Ast.Expr.ty []) (.lit (.natVal n))) => pure $ .ty n
+  | (.app (.app (.const `Ast.Expr.call []) lhs) rhs) => do
+    let lhs' ← from_expr lhs
+    let rhs' ← from_expr rhs
+
+    pure SKM`[(lhs' rhs')]
+  | .const `Ast.Expr.arr [] => pure SKM`[#~>]
   | .lam _ t body _     => do
     let t'    ← from_expr t
     let body' ← from_expr body
 
-    pure $ SKM'[λ t' => body']
+    pure $ SKM`[λ t' => body']
   | .forallE _ t body _ => do
     let t'    ← from_expr t
     let body' ← from_expr body
 
-    pure $ SKM'[∀ t', body']
+    pure $ SKM`[∀ t', body']
   | .app lhs rhs => do
     let lhs' ← from_expr lhs
     let rhs' ← from_expr rhs
 
-    pure $ SKM'[(lhs' rhs')]
+    pure $ SKM`[(lhs' rhs')]
   | e  => .error e
 
 def shift_down_from : ℕ →  IntermediateExpr → IntermediateExpr
   | j, v@(.var i)      => if i > j then (.var i.pred) else v
-  | j, (.call lhs rhs) => SKM'[(#(lhs.shift_down_from j)  #(rhs.shift_down_from j))]
-  | j, .lam  t b       => SKM'[λ #(t.shift_down_from j.succ) => #(b.shift_down_from j.succ)]
-  | j, .forE t b       => SKM'[∀ #(t.shift_down_from j.succ), #(b.shift_down_from j.succ)]
+  | j, (.call lhs rhs) => SKM`[(#(lhs.shift_down_from j)  #(rhs.shift_down_from j))]
+  | j, .lam  t b       => SKM`[λ #(t.shift_down_from j.succ) => #(b.shift_down_from j.succ)]
+  | j, .forE t b       => SKM`[∀ #(t.shift_down_from j.succ), #(b.shift_down_from j.succ)]
   | _, x               => x
 
 def free_in : ℕ → IntermediateExpr → Bool
   | j, (.var i) => i == j
   | j, (.call f x) => free_in j f || free_in j x
-  | j, SKM'[λ t => body] | j, SKM'[!(λ t => body)] => free_in j.succ t || free_in j.succ body
-  | j, SKM'[∀ t, body] | j, SKM'[!(∀ t, body)] => free_in j.succ t || free_in j.succ body
+  | j, SKM`[λ t => body] | j, SKM`[!(λ t => body)] => free_in j.succ t || free_in j.succ body
+  | j, SKM`[∀ t, body] | j, SKM`[!(∀ t, body)] => free_in j.succ t || free_in j.succ body
   | _, _ => false
 
 end IntermediateExpr
@@ -157,8 +157,8 @@ inductive AbstractMode where
   | e : AbstractMode
 
 def abstract : AbstractMode → List IntermediateExpr → ℕ → IntermediateExpr → MetaM IntermediateExpr
-  | mode, ctx@(t::_), j, e@SKM'[(lhs #(.var i))]
-  | mode, ctx@(t::_), j, e@SKM'[!(lhs #(.var i))] =>
+  | mode, ctx@(t::_), j, e@SKM`[(lhs #(.var i))]
+  | mode, ctx@(t::_), j, e@SKM`[!(lhs #(.var i))] =>
     if i == j && ¬ (lhs.free_in j) then
       pure $ lhs.shift_down_from j
     else do
@@ -168,16 +168,16 @@ def abstract : AbstractMode → List IntermediateExpr → ℕ → IntermediateEx
 
     if i == j then
       let pre := match mode with
-        | .e => SKM'[!S]
-        | .m => SKM'[!(M S)]
-      pure SKM'[!(((((pre ty) (ty ~> ty)) ty) ((K ty) (ty ~> ty))) ((K ty) ty))]
+        | .e => SKM`[!S]
+        | .m => SKM`[!(M S)]
+      pure SKM`[!(((((pre ty) (ty ~> ty)) ty) ((K ty) (ty ~> ty))) ((K ty) ty))]
     else
       let pre := match mode with
-        | .e => SKM'[K]
-        | .m => SKM'[(M K)]
-      pure SKM'[!(((pre ty) t) #(.var (if i > j then i.pred else i)))]
-  | mode, c@(t::_), j, e@SKM'[(lhs rhs)]
-  | mode, c@(t::_), j, e@SKM'[!(lhs rhs)] => do
+        | .e => SKM`[K]
+        | .m => SKM`[(M K)]
+      pure SKM`[!(((pre ty) t) #(.var (if i > j then i.pred else i)))]
+  | mode, c@(t::_), j, e@SKM`[(lhs rhs)]
+  | mode, c@(t::_), j, e@SKM`[!(lhs rhs)] => do
     if e.all_human_sk then
       pure e
     else
@@ -188,10 +188,10 @@ def abstract : AbstractMode → List IntermediateExpr → ℕ → IntermediateEx
       let t_rhs ← unwrap_intermediate r >>= (unwrap_check_error ∘ Expr.infer)
 
       let pre := match mode with
-        | .e => SKM'[!S]
-        | .m => SKM'[!(M S)]
+        | .e => SKM`[!S]
+        | .m => SKM`[!(M S)]
 
-      pure SKM'[!(((((pre #(.skm t_lhs)) #(.skm t_rhs)) t) l) r)]
+      pure SKM`[!(((((pre #(.skm t_lhs)) #(.skm t_rhs)) t) l) r)]
   | mode, c@(t::_), j, e => do
     let t_e ← unwrap_intermediate e >>= (unwrap_check_error ∘ Expr.infer)
 
@@ -199,10 +199,10 @@ def abstract : AbstractMode → List IntermediateExpr → ℕ → IntermediateEx
       pure e
     else
       let pre := match mode with
-        | .e => SKM'[!K]
-        | .m => SKM'[!(M K)]
+        | .e => SKM`[!K]
+        | .m => SKM`[!(M K)]
 
-      pure SKM'[!(((pre #(.skm t_e)) t) e)]
+      pure SKM`[!(((pre #(.skm t_e)) t) e)]
   | _, _, _, _ => throwError "context empty"
 
 def do_translate (ctx : List IntermediateExpr) (e : IntermediateExpr) : MetaM IntermediateExpr := do
@@ -210,24 +210,24 @@ def do_translate (ctx : List IntermediateExpr) (e : IntermediateExpr) : MetaM In
   | .some e => pure $ .skm e
   | _ => go ctx 0 e
   where go : List IntermediateExpr → ℕ → IntermediateExpr → MetaM IntermediateExpr
-    | ctx, lvl, SKM'[(λ t => body)]
-    | ctx, lvl, SKM'[!(λ t => body)] => do
+    | ctx, lvl, SKM`[(λ t => body)]
+    | ctx, lvl, SKM`[!(λ t => body)] => do
       let t'    ← go ctx lvl.succ t
       let body' ← go (t'::ctx) lvl.succ body
 
       abstract .e (t'::ctx) 0 body'
-    | ctx, lvl, SKM'[(∀ t, body)]
-    | ctx, lvl, SKM'[!(∀ t, body)] => do
+    | ctx, lvl, SKM`[(∀ t, body)]
+    | ctx, lvl, SKM`[!(∀ t, body)] => do
       let t'    ← go ctx lvl.succ t
       let body' ← go (t'::ctx) lvl.succ body
 
       abstract .m (t'::ctx) 0 body'
-    | ctx, lvl, SKM'[(lhs rhs)]
-    | ctx, lvl, SKM'[!(lhs rhs)] => do
+    | ctx, lvl, SKM`[(lhs rhs)]
+    | ctx, lvl, SKM`[!(lhs rhs)] => do
       let lhs' ← go ctx lvl lhs
       let rhs' ← go ctx lvl rhs
 
-      pure $ SKM'[(lhs' rhs')]
+      pure $ SKM`[(lhs' rhs')]
     | _, _, e => pure e
 
 elab "translate" e:term : term => do
@@ -238,7 +238,6 @@ elab "translate" e:term : term => do
     | .none   => throwError "couldn't convert back to Lean"
   | .error e => throwError s!"parsing failed: {repr e}"
 
-#eval Expr.infer $ translate (λ (x : Type 1) (y : Type 0) => x)
 
-
+example : (Expr.infer $ (translate (λ (x : SKM'[(M K)]) (y : SKM'[(M S)]) => x))) = .ok SKM[((M K) ~> ((M S) ~> (M K)))] := rfl
 
